dw/DeepWeb/Lib/NetworkAdapter.v
@@ -1,0 +1,42 @@
+(* Conversion from the effects used in the VST part
+   to the simplified version used by SimpleSpec. *)
+
+From DeepWeb.Free.Monad Require Import
+     Free Common.
+Import MonadNotations.
+Import SumNotations.
+Import NonDeterminismBis.
+
+From DeepWeb.Lib Require Import
+     NetworkInterface
+     SimpleSpec_NetworkInterface.
+
+Module N0 := NetworkInterface.
+Module N1 := SimpleSpec_NetworkInterface.
+
+Definition E0 := Common.nondetE +' failureE +' N0.networkE.
+
+Definition simplify_network' {E} `{nondetE -< E} `{N1.networkE -< E} :
+  forall X, E0 X -> M E X :=
+  fun _ e =>
+    match e with
+    | (| e ) =>
+      match e in N0.networkE X return M E X with
+      | N0.Listen _ => ret tt
+      | N0.Accept _ => N1.accept
+      | N0.RecvByte c => N1.recv_byte c
+      | N0.SendByte c b => N1.send_byte c b
+      | N0.Shutdown c => fail "not implemented"
+      end
+    | (| Fail reason |) => fail reason
+    | ( _Or ||) =>
+      match _Or in Common.nondetE X return M E X with
+      | Common.Or => or (ret false) (ret true)
+      end
+    end.
+
+Definition simplify_network {E} `{nondetE -< E} `{N1.networkE -< E} :
+  forall X, M E0 X -> M E X :=
+  fun _ => hom simplify_network'.
+
+Arguments simplify_network {E _ _} [X].
