dw/DeepWeb/Lib/SimpleSpec_NetworkInterface.v
@@ -1,0 +1,53 @@
+From Custom Require Import String.
+
+Require Import DeepWeb.Free.Monad.Free.
+Require Import DeepWeb.Free.Monad.Common.
+Import NonDeterminismBis.
+Import SumNotations.
+Import MonadNotations.
+
+Require Import DeepWeb.Lib.Util.
+
+(* A simple interface of server-side network effects. *)
+Inductive networkE : Type -> Type :=
+| Accept   : networkE connection_id
+| RecvByte : connection_id -> networkE byte
+| SendByte : connection_id -> byte -> networkE unit
+.
+
+(* A server is a program with internal nondeterminism and
+   external network effects. *)
+Definition serverE := nondetE +' networkE.
+
+(* The server itree type. *)
+Definition itree_server := M (nondetE +' networkE) unit.
+
+Definition accept {E} `{networkE -< E}
+  : M E connection_id := embed Accept.
+
+Definition recv_byte {E} `{networkE -< E}
+  : connection_id -> M E byte := embed RecvByte.
+
+Definition send_byte {E} `{networkE -< E}
+  : connection_id -> byte -> M E unit := embed SendByte.
+
+(* Receive up to [n] bytes. *)
+Fixpoint recv {E} `{networkE -< E} `{nondetE -< E}
+           (c : connection_id) (n : nat) : M E bytes :=
+  match n with
+  | O => ret ""
+  | S n =>
+    b <- recv_byte c;;
+    bs <- recv c n;;
+    ret (b ::: bs)
+  end%string.
+
+(* Receive a bytestring of length [n] exactly. *)
+Definition recv_full {E} `{networkE -< E}
+           (c : connection_id) (n : nat) : M E bytes :=
+  replicate_bytes n (recv_byte c).
+
+(* Send all bytes in a bytestring. *)
+Fixpoint send {E} `{networkE -< E}
+         (c : connection_id) (bs : bytes) : M E unit :=
+  for_bytes bs (send_byte c).
