dw/DeepWeb/Lib/Socket.v
@@ -1,2 +1,3 @@
+Require Export DeepWeb.Lib.Util.
 Require Export DeepWeb.Lib.SocketInterface.
 Require Export DeepWeb.Lib.SocketConstants.
