dw/DeepWeb/Lib/Util.v
@@ -1,0 +1,100 @@
+From Custom Require Import
+     Monad String List.
+Import MonadNotations.
+
+From QuickChick Require Import
+     Decidability Show.
+
+From DeepWeb.Free Require Import
+     Monad.Free.
+
+(* Bytes *)
+
+(* We use Coq's standard [string] type to use its
+   pretty-printing niceness. *)
+
+(* Single byte *)
+Definition byte : Type := Ascii.ascii.
+
+(* Bytestring *)
+Definition bytes : Type := String.string.
+
+(* Iterate a byte-producing process [n] times. *)
+Fixpoint replicate_bytes {E} (n : nat) (get_byte : M E byte) :
+  M E bytes :=
+  match n with
+  | O => ret ""
+  | S n =>
+    b <- get_byte;;
+    bs <- replicate_bytes n get_byte;;
+    ret (b ::: bs)
+  end%string.
+
+(* Loop over each byte. *)
+Fixpoint for_bytes {E} (bs : bytes) (eat_byte : byte -> M E unit) :
+  M E unit :=
+  match bs with
+  | "" => ret tt
+  | b ::: bs => eat_byte b;; for_bytes bs eat_byte
+  end%string.
+
+(* Get a null-terminated sequence of bytes, excluding the zero-byte
+   delimiter. Loops infinitely if there is no zero-byte. *)
+Definition get_str {E} (get_byte : M E byte) : M E bytes :=
+  (cofix get_str' (mk_bytes : bytes -> bytes) : M E bytes :=
+     bindM get_byte (fun b =>
+     if b = "000"%char ? then
+       ret (mk_bytes "")%string
+     else
+       Tau (get_str' (fun bs => mk_bytes (b ::: bs)%string))))
+    (fun bs => bs).
+
+(* Loop over each byte and an extra null byte at the end. *)
+Fixpoint for_str {E} (bs : bytes) (eat_byte : byte -> M E unit) :
+  M E unit :=
+  match bs with
+  | "" => eat_byte "000"%char
+  | b ::: bs => eat_byte b;; for_str bs eat_byte
+  end%string.
+
+(* Network *)
+
+Require Import ZArith.
+
+Inductive connection_id : Type := Connection (c : nat).
+
+Record endpoint_id : Type := Endpoint
+  { port_number : Z;
+  }.
+
+Definition eqb_connection_id :
+  forall c1 c2 : connection_id, {c1 = c2} + {c1 <> c2}.
+Proof. intros [] []; dec_eq. Defined.
+
+Instance Eq_connection_id : Eq connection_id :=
+  { dec_eq := eqb_connection_id }.
+
+Instance Eq_endpoint_id : Eq endpoint_id := {}.
+Proof. intros; dec_eq. Defined.
+
+Instance Show_connection_id : Show connection_id :=
+  { show := fun '(Connection c) => show c }.
+
+Instance Show_endpoint_id : Show endpoint_id :=
+  { show := fun '(Endpoint p) => show p }.
+
+Module TestDefault.
+
+(* Dummy value for the endpoint (ignored). *)
+Definition endpoint : endpoint_id
+  := Endpoint 0.
+
+(* A short buffer size for easier testing. *)
+Definition buffer_size : nat
+  := 3.
+
+(* "000" *)
+Definition init_message : bytes
+  := repeat_string "0"%char buffer_size.
+
+End TestDefault.
