dw/DeepWeb/Proofs/Vst/AppLib.v
@@ -1,215 +1,528 @@
 Require Import String.
 
-From DeepWeb.Proofs.Vst
-     Require Import VstInit.
+From DeepWeb.Spec
+     Require Import Vst.MainInit Vst.AppLogic Vst.SocketSpecs
+     Vst.Representation Swap_CLikeSpec.
 
-Require Import DeepWeb.Spec.ITreeSpec.
+From DeepWeb.Lib
+     Require Import VstLib.
 
 Open Scope list.
 Open Scope logic.
 
+Import SockAPIPred.
+
 Set Bullet Behavior "Strict Subproofs".
 
-Section Basic_Extensions.
-  Lemma filter_app: forall {A : Type} f (l1 l2 : list A),
-    filter f (l1 ++ l2) = filter f l1 ++ filter f l2.
-  Proof.
-    induction l1; intros; trivial.
-    simpl.
-    destruct (f a); trivial.
-    simpl.
-    f_equal.
-    apply IHl1.
-  Qed.
-
-  (*
-Lemma In_preserved_by_map:
-  forall {A B} (f : A -> B) (l1 l2 : list A),
-    incl l1 l2 ->
-    (forall y, In y (map f l1) -> In y (map f l2)).
-Proof.
-  intros A B f l1 l2 HIncl y HIn_map.
-  apply list_in_map_inv in HIn_map.
-  destruct HIn_map as [x [y_eq x_in]]; subst.
-  apply in_map.
-  unfold incl in HIncl; apply HIncl.
-  assumption.
-Qed.
-   *)
-
-  Lemma filter_incl:
-    forall {A} (p : A -> bool) l, incl (filter p l) l.
-  Proof.
-    unfold incl.
-    intros ? ? ? ? HIn.
-    rewrite filter_In in HIn.
-    destruct HIn; assumption.
-  Qed.
-
-  Lemma projected_filter_reflects_cond:
-    forall {X Y} (f : X -> Y) (cond : X -> bool) (l : list X) (x : X) (y : Y),
-      y = f x ->
-      In x l -> 
-      In y (map f (filter cond l)) ->
-      NoDup (map f l) ->
-      cond x = true.
-  Proof.
-    intros X Y f cond.
-    induction l as [| a xs]; intros x y y_eq x_in y_in HNoDup;
-      subst y; auto.
-    destruct (cond x) eqn:Hcond; auto.
-    exfalso.
-    simpl in x_in.
-    destruct x_in as [x_in_head | x_in_tail].
-    - subst a.
-      simpl in y_in.
-      rewrite Hcond in y_in; simpl in y_in.
-      pose proof (list_in_map_inv _ _ _ y_in) as H.
-      destruct H as [x' [image_eq x'_in]].
-      assert (In x' xs) as x'_in_tail by (eapply filter_incl; eassumption).
-      simpl in HNoDup.
-      rewrite NoDup_cons_iff in HNoDup.
-      destruct HNoDup.
-      apply in_map with (f0 := f) in x'_in_tail.
-      rewrite image_eq in *.
-      tauto.
-
-    - simpl in HNoDup.
-      rewrite NoDup_cons_iff in HNoDup.
-      destruct HNoDup.
-      assert (In (f x) (map f xs)) as fx_in_tail
-          by (apply in_map; auto).
-
-      simpl in y_in.
-      destruct (cond a).
-      + simpl in y_in.
-        destruct y_in as [fa_fx | fx_in_filtered_tail];
-          [rewrite fa_fx in *; tauto |].
-        apply IHxs with (x := x) in fx_in_filtered_tail; auto.
-        rewrite Hcond in *; discriminate.
-      + apply IHxs with (x := x) in y_in; auto.
-        rewrite Hcond in *; discriminate.
-  Qed.
-
-  Lemma same_key_preserves_NoDup:
-    forall (T : Type) (g : T -> Z) (t t' : T) (prefix suffix : list T),
-      g t = g t' ->
-      NoDup (map g (prefix ++ t :: suffix)) ->
-      NoDup (map g (prefix ++ t' :: suffix)).
-  Proof.
-    intros T g t t' prefix suffix Heq HNoDup.
-    rewrite map_app in *.
-    simpl in *.
-    rewrite <- Heq.
-    trivial.
-  Qed.
-
-End Basic_Extensions.
-
-
-Section Interaction_Tree.
-  
-  Lemma replace_eq_given_discriminator
-        {A : Type} (p1 p2: A -> bool) (g : A -> nat):
-    forall (n : nat),
-      (forall y, p1 y = true -> g y = n /\ p2 y = true) -> 
-      forall (l : list A) (x : A),
-        ~In n (map g (filter p2 l)) ->
-        replace_when p1 x l = l.
-  Proof.
-    intros n Hdiscriminate.
-    induction l as [| a l]; intros x n_not_in; auto.
-    simpl.
-    destruct (p1 _) eqn:p1_test; [| f_equal; apply IHl; try assumption].
-    2 : {
-      unfold not; intros Hcontra.
-      simpl in n_not_in.
-      destruct (p2 _); auto; simpl in n_not_in.
-      destruct n_not_in; auto.
-    }
-
-    apply Hdiscriminate in p1_test.
-    destruct p1_test as [g_a p2_test].
-    revert n_not_in.
-    simpl.
-    rewrite p2_test.
-    simpl.
-    rewrite g_a.
-    intros; tauto.
-  Qed.        
-
-  Lemma replace_when_NoDup {A : Type} (p1 p2: A -> bool) (g : A -> nat):
-    forall (n : nat),
-      (forall y, p1 y = true <-> g y = n /\ p2 y = true) ->
-      forall (prefix suffix : list A) (x x' : A),
-        g x = n /\ p2 x = true ->
-        ~In (g x) (map g (filter p2 (prefix ++ suffix))) ->
-        replace_when p1 x' (prefix ++ x :: suffix) = prefix ++ x' :: suffix.
-  Proof.
-    intros n tests_equal prefix suffix x x' [g_x p2_x]
-           n_not_in.
-    assert (forall y, p1 y = true -> g y = n /\ p2 y = true)
-      as p1_p2.
-    {
-      intros; apply tests_equal; assumption.
-    }
-
-    assert (forall y, g y = n -> p2 y = true -> p1 y = true)
-      as p2_p1.
-    {
-      intros; apply tests_equal; auto.
-    }
-    
-    revert dependent prefix.
-    induction prefix as [| a prefix]; intros n_not_in;
-      rewrite g_x in *.
-    { simpl.
-      simpl in n_not_in.
-      destruct (p1 _) eqn:p1_test.
-      - f_equal.
-        eapply replace_eq_given_discriminator; eauto.
-      - pose proof (p2_p1 _ g_x p2_x).
-        rewrite p1_test in *; discriminate.
-    } 
-
-    simpl.
-    destruct (p1 _) eqn:p1_test.
-    - destruct (p1_p2 _ p1_test) as [g_a p2_a].
-      revert n_not_in.
-      simpl.
-      rewrite p2_a.
-      simpl.
-      intros; tauto.
-    - f_equal.
-      apply IHprefix.
-      unfold not.
-      intros Hcontra.
-      
-      assert (In n (map g (filter p2 [a]))
-              \/ In n (map g (filter p2 (prefix ++ suffix))))
-        as H by auto.
-      apply in_or_app in H.
-      rewrite <- map_app in H.
-      rewrite <- filter_app in H.
-      simpl app in H.
-      tauto.
-  Qed.
-
-  Lemma conditional_id_iff {A : Type} (cond : A -> bool) (id : A -> nat):
-    forall (x : A) (n : nat),
-      (if cond x then (id x =? n)%nat else false) = true <->
-      id x = n /\ cond x = true.
+Section Consistent_Facts.
+  Lemma consistent_connection_not_closed:
+    forall (buffer_size : Z) (st : SocketMap) (conn : connection) (fd: sockfd), 
+      consistent_state buffer_size st (conn, fd) ->
+      lookup_socket st fd <> ClosedSocket.
   Proof.
     intros.
-    split. 
-    - destruct (cond x); split; auto.
-      + rewrite Nat.eqb_eq in H.
-        assumption.
-      + discriminate.
-    - intros [id_n cond_x].
-      rewrite cond_x.
-      rewrite Nat.eqb_eq.
-      assumption.
+    inversion H; subst; simpl in *; unfold not; intros;
+      try (match goal with
+           | [H1: lookup_socket _ _ = _, H2 : lookup_socket _ _ = _ |- _] =>
+             rewrite H2 in H1; inversion H1
+           end).
+    match goal with
+    | [H1: lookup_socket _ _ = _ \/ _, H2: lookup_socket _ _ = _ |- _ ] =>
+      destruct H1 as [Open | Open];
+        rewrite H2 in Open; inversion Open
+    end.
   Qed.
 
-End Interaction_Tree.
+  Lemma consistent_connection_not_listening:
+    forall (buffer_size : Z) (st : SocketMap) (conn : connection) (fd : sockfd), 
+      consistent_state buffer_size st (conn, fd) ->
+      (forall addr, lookup_socket st fd <> ListeningSocket addr).
+  Proof.
+    intros.
+    inversion H; subst; simpl in *; unfold not; intros;
+      try (match goal with
+           | [H1: lookup_socket _ _ = _, H2 : lookup_socket _ _ = _ |- _] =>
+             rewrite H2 in H1; inversion H1
+           end).
+    match goal with
+    | [H1: lookup_socket _ _ = _ \/ _, H2: lookup_socket _ _ = _ |- _ ] =>
+      destruct H1 as [Open | Open];
+        rewrite H2 in Open; inversion Open
+    end.
+  Qed.
+
+  Lemma consistent_RECVING_SENDING_connected:
+    forall (buffer_size : Z) (st : SocketMap) (conn : connection) (fd : sockfd), 
+      consistent_state buffer_size st (conn, fd) ->
+      conn_state conn = RECVING \/ conn_state conn = SENDING -> 
+      lookup_socket st fd = ConnectedSocket (conn_id conn).
+  Proof.
+    intros ? ? ? ? H Hconn_state.
+    inversion H; subst; simpl in *; auto.
+    destruct Hconn_state; discriminate.
+  Qed.    
+
+  Lemma consistent_connection_fd_bound:
+    forall (buffer_size : Z) (st : SocketMap) (conn : connection) (fd : sockfd), 
+      consistent_state buffer_size st (conn, fd) ->
+      0 <= descriptor fd < FD_SETSIZE.
+  Proof.
+    intros.
+    destruct conn.
+    simpl.
+    inversion H;
+      inversion H4;
+      split; try apply fd_bound; auto; apply (is_descriptor fd).
+  Qed.
+
+  Lemma consistent_connection_response_bytes_sent_bound:
+    forall (buffer_size : Z) (st : SocketMap) (conn : connection) (fd : sockfd), 
+      consistent_state buffer_size st (conn, fd) ->
+      conn_state conn = SENDING ->
+      0 <= conn_response_bytes_sent conn
+      <= Zlength (val_of_string (conn_response conn)).
+  Proof.
+    intros ? ? conn ? Hconsistent ?.
+    inversion Hconsistent; subst conn; simpl; split;
+      try omega; [apply Zlength_nonneg |..].
+  Qed.
+  
+End Consistent_Facts.
+
+Section Preservation.
+  
+  Lemma update_preserves_frame_consistency:
+    forall (buffer_size : Z) (st1 st2 : SocketMap)
+      (fd : sockfd)
+      (new_state : socket_status)
+      (connections : list (connection * sockfd * val)),
+      ~In (descriptor fd) (map descriptor (map proj_fd connections)) ->
+      st2 = update_socket_state st1 fd new_state ->
+      Forall (fun '(conn, fd, _) =>
+                consistent_state buffer_size st1 (conn, fd)) connections ->
+      Forall (fun '(conn, fd, _) =>
+                consistent_state buffer_size st2 (conn, fd)) connections.
+  Proof.
+    intros buffer_size
+           st1 st2 fd new_state connections not_in st2_eq all_consistent.
+    rewrite Forall_forall in *.
+    intros [[conn conn_fd] ptr] conn_in.
+    assert (descriptor fd <> descriptor conn_fd) as Hneq.
+    { unfold not.
+      intros Heq.
+      apply not_in.
+      rewrite Heq.
+      apply List.in_map.
+      change conn_fd with (proj_fd (conn, conn_fd, ptr)).
+      apply List.in_map.
+      trivial.
+    }
+    
+    specialize (all_consistent (conn, conn_fd, ptr) conn_in).
+    simpl in all_consistent.
+
+    inversion all_consistent;
+      [ eapply Consistent_RECVING; eauto
+      | eapply Consistent_SENDING; eauto
+      | eapply Consistent_DELETED; eauto];
+      rewrite st2_eq;
+      repeat rewrite lookup_update_socket_neq;
+      trivial.
+  Qed.
+  
+End Preservation.
+
+Section Step_Preservation.
+  
+  Lemma recv_step_preserves_descriptors:
+    forall (buffer_size : Z) (conn conn' : connection) (fd fd' : sockfd)
+      (st st' : SocketMap) (msg_in_store msg_in_store' : string),
+      recv_step buffer_size
+                (conn, fd, st, msg_in_store)
+                (conn', fd', st', msg_in_store') ->
+      fd = fd'.
+  Proof.
+    intros.
+    inversion H;
+      match goal with
+      | [H1: conn' = _ |- _] =>
+        rewrite H1; reflexivity
+      | _ =>
+        reflexivity
+      end.
+  Qed.
+
+  Lemma send_step_preserves_descriptors:
+    forall (conn conn' : connection) (fd fd' : sockfd)
+      (st st' : SocketMap),
+      send_step (conn, fd, st) (conn', fd', st') ->
+      fd = fd'.
+  Proof.
+    intros.
+    inversion H;
+      match goal with
+      | [H1: conn' = _ |- _] =>
+        rewrite H1; reflexivity
+      | _ =>
+        reflexivity
+      end.
+  Qed.
+
+  Lemma recv_step_preserves_consistency:
+    forall buffer_size conn fd st conn' fd' st' msg_in_store msg_in_store',
+      recv_step buffer_size
+                (conn, fd, st, msg_in_store)
+                (conn', fd', st', msg_in_store') ->
+      consistent_state buffer_size st (conn, fd) ->
+      consistent_state buffer_size st' (conn', fd').
+  Proof.
+    intros ? conn fd st conn' fd' st' msg_in_store msg_in_store'
+           Hrecv Hconsistent.
+    inversion Hrecv.
+    - (* Conn_RECVING_RECVING *)
+      inversion Hconsistent.
+      all:
+        subst;
+        simpl in *;
+        match goal with
+        | [H: _ = RECVING |- _] =>
+          try inversion H
+        end.
+      + eapply Consistent_RECVING;
+          [eauto | subst; auto..].
+    - (* Conn_RECVING_SENDING *)
+      inversion Hconsistent.
+      all:
+        subst;
+        simpl in *;
+        match goal with
+        | [H: _ = RECVING |- _] =>
+          try inversion H
+        end.
+      + eapply Consistent_SENDING;
+          [eauto | reflexivity | subst; auto | eauto |].
+        split; [omega | apply Zlength_nonneg].
+    - (* Conn_RECVING_EOF *)
+      inversion Hconsistent.
+      all:
+        subst;
+        simpl in *;
+        match goal with
+        | [H: _ = RECVING |- _] =>
+          try inversion H
+        end.    
+      + eapply Consistent_DELETED;
+          [eauto | subst; auto..].
+        rewrite lookup_update_socket_eq; auto.
+        split; try omega; apply Zlength_nonneg.
+    - (* Conn_RECVING_Id *)
+      subst; auto.
+  Qed.    
+
+  Lemma send_step_preserves_consistency:
+    forall buffer_size conn fd st conn' fd' st',
+      send_step (conn, fd, st) (conn', fd', st') ->
+      consistent_state buffer_size st (conn, fd) ->
+      consistent_state buffer_size st' (conn', fd').
+  Proof.
+    intros ? conn fd st conn' fd' st' Hsend Hconsistent.
+    inversion Hsend.
+    - (* Conn_SENDING_SENDING *)
+      inversion Hconsistent.
+      all:
+        subst;
+        simpl in *;
+        match goal with
+        | [H: _ = SENDING |- _] =>
+          try inversion H
+        end.
+      + eapply Consistent_SENDING;
+          [eauto | subst; auto..].
+        subst total_num_bytes_sent response_length.
+        split; omega.
+    - (* Conn_SENDING_RECVING *)
+      inversion Hconsistent.
+      all:
+        subst;
+        simpl in *;
+        match goal with
+        | [H: _ = SENDING |- _] =>
+          try inversion H
+        end.
+      + eapply Consistent_RECVING;
+          [eauto | subst; auto..].
+    - (* Conn_SENDING_Fail *)
+      eapply Consistent_DELETED with (client_fd := fd');
+        [| subst; auto .. ].
+      + inversion Hconsistent; subst; trivial.
+      + match goal with
+        | [H: st' = _ \/ _ |- _] =>
+          destruct H; 
+            [inversion Hconsistent; subst; auto |]
+        end.
+        subst; auto.
+        left; unfold update_socket_state.
+        simpl.
+        assert ((descriptor fd' =? descriptor fd') = true)
+          by (rewrite Z.eqb_eq; reflexivity).
+        rewrite H; reflexivity.
+      + inversion Hconsistent; subst; simpl; split;
+          try omega; apply Zlength_nonneg.
+  Qed.
+  
+  Lemma recv_step_preserves_frame_consistency:
+    forall (buffer_size : Z) (st1 st2 : SocketMap)
+      (prefix suffix : list (connection * sockfd * val))
+      (conn1 conn2 : connection)
+      (fd : sockfd) (ptr : val)
+      (msg_in_store1 msg_in_store2 : string),
+      Forall (fun '(conn, fd, ptr) =>
+                consistent_state buffer_size st1 (conn, fd))
+             prefix ->
+      Forall (fun '(conn, fd, ptr) =>
+                consistent_state buffer_size st1 (conn, fd))
+             suffix ->
+      NoDup
+        (map descriptor
+             (map proj_fd (prefix ++ (conn1, fd, ptr) :: suffix))) ->
+      recv_step buffer_size
+                (conn1, fd, st1, msg_in_store1)
+                (conn2, fd, st2, msg_in_store2) ->
+      Forall (fun '(conn, fd, ptr) =>
+                consistent_state buffer_size st2 (conn, fd))
+             prefix /\
+      Forall (fun '(conn, fd, ptr) =>
+                consistent_state buffer_size st2 (conn, fd))
+             suffix.
+  Proof.
+    intros ? st1 st2 prefix suffix conn1 conn2 fd ptr
+           msg_in_store1 msg_in_store2
+           prefix_consistent suffix_consistent
+           HNoDup Hstep.
+    pose proof (recv_step_preserves_descriptors _ _ _ _ _ _ _ _ _ Hstep).
+    repeat rewrite map_app in HNoDup.
+    simpl in HNoDup.
+    apply NoDup_remove_2 in HNoDup.
+    rewrite in_app in HNoDup.
+    apply Classical_Prop.not_or_and in HNoDup.
+    destruct HNoDup.
+    
+    split; inversion Hstep;
+      subst.
+    
+    all:
+      eapply update_preserves_frame_consistency;
+      [ eassumption
+      | rewrite <- update_socket_id; auto
+      | trivial].
+
+    all:
+      eapply update_preserves_frame_consistency;
+      [ eassumption
+      | reflexivity
+      | assumption].
+  Qed.
+
+  Lemma send_step_preserves_frame_consistency:
+    forall (buffer_size : Z) (st1 st2 : SocketMap)
+      (prefix suffix : list (connection * sockfd * val))
+      (conn1 conn2 : connection)
+      (fd : sockfd) (ptr : val),
+      Forall (fun '(conn, fd, ptr) =>
+                consistent_state buffer_size st1 (conn, fd))
+             prefix ->
+      Forall (fun '(conn, fd, ptr) =>
+                consistent_state buffer_size st1 (conn, fd))
+             suffix ->
+      NoDup
+        (map descriptor (map proj_fd (prefix ++ (conn1, fd, ptr) :: suffix))) ->
+      send_step (conn1, fd, st1) (conn2, fd, st2) ->
+      Forall (fun '(conn, fd, ptr) =>
+                consistent_state buffer_size st2 (conn, fd))
+             prefix /\
+      Forall (fun '(conn, fd, ptr) =>
+                consistent_state buffer_size st2 (conn, fd))
+             suffix.
+  Proof.
+    intros ? st1 st2 prefix suffix conn1 conn2 fd ptr
+           prefix_consistent suffix_consistent
+           HNoDup Hstep.
+    pose proof (send_step_preserves_descriptors _ _ _ _ _ _ Hstep).
+    repeat rewrite map_app in HNoDup.
+    simpl in HNoDup.
+    apply NoDup_remove_2 in HNoDup.
+    rewrite in_app in HNoDup.
+    apply Classical_Prop.not_or_and in HNoDup.
+    destruct HNoDup.
+    
+    split; inversion Hstep;
+      subst.
+    
+    all:
+      eapply update_preserves_frame_consistency;
+      [ eassumption
+      | rewrite <- update_socket_id; auto
+      | trivial].
+
+    all:
+      match goal with
+      | [H: _ \/ _ |- _] =>
+        destruct H; subst
+      end;
+      eapply update_preserves_frame_consistency;
+      [ eassumption
+      | apply update_socket_id
+      | trivial
+      | eassumption
+      | reflexivity
+      | trivial
+      ].
+  Qed.
+
+  Lemma recv_step_preserves_frame_lookup:
+    forall buffer_size conn conn' fd st st' msg_in_store msg_in_store' frame_fd,
+      recv_step buffer_size
+                (conn, fd, st, msg_in_store)
+                (conn', fd, st', msg_in_store') ->
+      descriptor frame_fd <> descriptor fd ->
+      lookup_socket st frame_fd = lookup_socket st' frame_fd.
+  Proof.
+    intros ? ? ? ? ? ? ? ? ? Hstep Hdescr.
+    inversion Hstep; subst; auto.
+    rewrite lookup_update_socket_neq; auto.
+  Qed.
+
+  Lemma send_step_preserves_frame_lookup:
+    forall conn conn' fd st st' frame_fd,
+      send_step (conn, fd, st) (conn', fd, st') ->
+      descriptor frame_fd <> descriptor fd ->
+      lookup_socket st frame_fd = lookup_socket st' frame_fd.
+  Proof.
+    intros ? ? ? ? ? ? Hstep Hdescr.
+    inversion Hstep; subst; auto.
+    match goal with
+    | [H: _ \/ _ |- _] =>
+      destruct H; subst; auto
+    end.
+    rewrite lookup_update_socket_neq; auto.
+  Qed.
+  
+  Lemma recv_step_preserves_conn_ids:
+    forall (buffer_size : Z) (conn conn' : connection) (fd fd' : sockfd)
+      (st st' : SocketMap) (msg_in_store msg_in_store' : string),
+      recv_step buffer_size
+                (conn, fd, st, msg_in_store)
+                (conn', fd', st', msg_in_store') ->
+      conn_id conn = conn_id conn'.
+  Proof.
+    intros.
+    inversion H;
+      match goal with
+      | [H1: conn' = _ |- _] =>
+        rewrite H1; reflexivity
+      | _ =>
+        reflexivity
+      end.
+  Qed.
+
+  Lemma send_step_preserves_conn_ids:
+    forall (conn conn' : connection) (fd fd' : sockfd)
+      (st st' : SocketMap),
+      send_step (conn, fd, st) (conn', fd', st') ->
+      conn_id conn = conn_id conn'.
+  Proof.
+    intros.
+    inversion H;
+      match goal with
+      | [H1: conn' = _ |- _] =>
+        rewrite H1; reflexivity
+      | _ =>
+        reflexivity
+      end.
+  Qed.
+
+End Step_Preservation.
+
+Section New_Descriptor.
+  
+  Lemma new_descriptor_is_distinct: forall buffer_size st connections fd,
+    Forall (fun '(conn, fd, _) =>
+              consistent_state buffer_size st (conn, fd)) connections ->
+    lookup_socket st fd = ClosedSocket ->
+    ~ In (descriptor fd) (map descriptor (map proj_fd connections)).
+  Proof.
+    intros ? st connections fd all_consistent lookup_closed.
+    unfold not; intros Hcontra.
+    apply list_in_map_inv in Hcontra.
+    destruct Hcontra
+      as [fd' [fd'_eq fd'_in]].
+    apply list_in_map_inv in fd'_in.
+    destruct fd'_in
+      as [[[conn' fd''] ptr] [fd''_eq conn_in]].
+    simpl in fd''_eq; subst fd''.
+    rewrite Forall_forall in all_consistent;
+      apply all_consistent in conn_in.
+    apply consistent_connection_not_closed in conn_in.
+    apply lookup_descriptor with (api_st := st) in fd'_eq.
+    rewrite lookup_closed in fd'_eq.
+    rewrite <- fd'_eq in conn_in.
+    tauto.
+  Qed.
+  
+  Lemma new_descriptor_preserves_consistency:
+    forall (buffer_size : Z) (st1 st2 : SocketMap)
+      (client_conn : connection_id)
+      (client_fd : sockfd)
+      (connections : list (connection * sockfd * val)),
+      lookup_socket st1 client_fd = ClosedSocket ->
+      st2 = update_socket_state st1 client_fd
+                                (ConnectedSocket client_conn) ->
+      Forall (fun '(conn, fd, _) =>
+                consistent_state buffer_size st1 (conn, fd)) connections ->
+      Forall (fun '(conn, fd, _) =>
+                consistent_state buffer_size st2 (conn, fd)) connections.
+  Proof.
+    intros.
+    eapply update_preserves_frame_consistency; eauto.
+    eapply new_descriptor_is_distinct; eauto.
+  Qed.
+
+  
+  Lemma new_descriptor_preserves_NoDup:
+    forall (buffer_size : Z) (st : SocketMap) (new_fd : sockfd)
+      (connections : list (connection * sockfd * val)) (descriptors : list Z),
+      lookup_socket st new_fd = ClosedSocket ->
+      Forall (fun '(conn, fd, _) => 
+                consistent_state buffer_size st (conn, fd))
+             connections ->
+      descriptors = map descriptor (map proj_fd connections) ->
+      NoDup descriptors ->
+      NoDup ((descriptor new_fd) :: descriptors).
+  Proof.
+    intros.
+    rewrite NoDup_cons_iff.
+    subst.
+    split; [eapply new_descriptor_is_distinct; eauto |].
+    assumption.
+  Qed.
+  
+End New_Descriptor.
+
+Lemma fd_in_filtered_implies_conn_state:
+  forall (l : list (connection * sockfd * val)) conn fd ptr st filtered,
+    In (conn, fd, ptr) l -> 
+    filtered = map proj_fd (filter (has_conn_state st) l) ->
+    In (descriptor fd) (map descriptor filtered) ->
+    NoDup (map descriptor (map proj_fd l)) ->
+    has_conn_state st conn = true.
+Proof.
+  intros l ? ? ? ? ? ? ? in_filtered HNoDup.
+  change (descriptor fd)
+    with (descriptor (proj_fd (conn, fd, ptr))) in in_filtered.
+  subst filtered.
+  rewrite map_map in in_filtered.
+  apply projected_filter_reflects_cond with (x := (conn, fd, ptr))
+    in in_filtered; auto.
+  rewrite <- map_map.
+  assumption.
+Qed.
