dw/DeepWeb/Proofs/Vst/VerifLib.v
@@ -1,0 +1,663 @@
+Require Import String.
+
+From DeepWeb.Spec
+     Require Import Swap_CLikeSpec
+     Vst.SocketSpecs Vst.MainInit Vst.MonadExports.
+
+From DeepWeb.Lib 
+     Require Import VstLib.
+
+Import TracePred.
+Import SockAPIPred.
+
+Open Scope logic.
+Open Scope list.
+
+Definition malloc_tokens (t : type) (ptrs : list val) :=
+  fold_right (fun ptr a => sepcon a (malloc_token Tsh t ptr)) emp ptrs.
+
+Lemma cons_malloc_tokens (t : type) (ptrs : list val) (ptr : val):
+  malloc_tokens t ptrs * malloc_token Tsh t ptr
+  = malloc_tokens t (ptr :: ptrs).
+Proof.
+  unfold malloc_tokens.
+  rewrite fold_right_cons.
+  reflexivity.
+Qed.
+
+Lemma split_data_app:
+  forall (n1 n2 : Z) (prefix suffix : list val) (ptr : val)
+    (sh : share),
+    0 <= n1 <= n2 ->
+    Zlength prefix = n1 ->
+    Zlength suffix = n2 - n1 ->
+    data_at sh (Tarray tuchar n2 noattr) (prefix ++ suffix) ptr =              
+    data_at sh (Tarray tuchar n1 noattr)
+            prefix ptr *
+    data_at sh (Tarray tuchar (n2 - n1) noattr)
+            suffix (field_address0 (Tarray tuchar n2 noattr)
+                                   [ArraySubsc n1] ptr).
+Proof.
+  intros n1 n2 prefix suffix ptr sh [? ?] prefix_len suffix_len.
+  remember (prefix ++ suffix) as buffer.
+  assert (prefix = sublist 0 n1 buffer) as prefix_eq.
+  {
+    rewrite Heqbuffer.
+    rewrite sublist_app1; [| omega..].
+    rewrite <- prefix_len.
+    rewrite sublist_same; auto.
+  }
+  assert (suffix = sublist n1 n2 buffer) as suffix_eq.
+  {
+    rewrite Heqbuffer.
+    rewrite sublist_app2; [| omega].
+    rewrite sublist_same; [auto | omega |].
+    rewrite prefix_len.
+    auto.
+  }
+  rewrite prefix_eq.
+  rewrite suffix_eq.
+  apply split2_data_at_Tarray_tuchar; [omega |].
+  subst; rewrite Zlength_app; omega.
+Qed.
+
+Lemma data_at__Tarray_Vundef:
+  forall n sh attr ptr,
+    data_at sh (Tarray tuchar n attr)
+            (list_repeat (Z.to_nat n) Vundef)
+            ptr
+    = data_at_ sh (Tarray tuchar n attr) ptr.
+Proof.
+  intros.
+  unfold data_at_.
+  unfold field_at_.
+  unfold default_val.
+  simpl.
+  reflexivity.
+Qed.
+
+Lemma split_data_with_undefined_tail:
+  forall (n1 n2 : Z) (prefix suffix : list val) (ptr : val) (sh : share),
+    0 <= n1 <= n2 ->
+    n1 = Zlength prefix ->
+    suffix = list_repeat (Z.to_nat (n2 - n1)) Vundef ->
+    data_at sh (Tarray tuchar n2 noattr) (prefix ++ suffix) ptr =              
+    data_at sh (Tarray tuchar n1 noattr)
+            prefix ptr *
+    data_at_ sh (Tarray tuchar (n2 - n1) noattr)
+             (field_address0 (Tarray tuchar n2 noattr)
+                             [ArraySubsc n1] ptr).
+Proof.
+  intros.
+  rewrite <- data_at__Tarray_Vundef.
+  rewrite H1.
+  pose proof split_data_app as Hsplit.
+  unfold tarray in Hsplit.
+  rewrite split_data_app with (n1 := n1); auto.
+  rewrite Zlength_list_repeat; omega.
+Qed.
+
+Module Auto_DB.
+
+  Hint Rewrite <- val_of_string_app : sublist_supp.
+  Hint Rewrite <- Zlength_app : sublist_supp.
+
+  (* Conversion from Nat to Z *)
+  Hint Rewrite Z2Nat.id using (subst; simpl; try omega) : sublist_supp.
+  Hint Rewrite Nat2Z.id : sublist_supp.
+  Hint Rewrite Nat2Z.inj_le using (subst; simpl; try omega) : sublist_supp.
+
+  (* String *)
+  Hint Rewrite <- Zlength_val_string_len : sublist_supp.
+  Hint Rewrite substring_sublist : sublist_supp.
+  (* Warning: May be over-aggressive; assumes that everything is within 
+     bounds *)
+  Hint Rewrite (@sublist_skip val)
+       using (subst; simpl; try omega) : sublist_supp.
+  Hint Rewrite (@Zlength_skipn val) : sublist_supp.
+  Hint Rewrite Zmax0r using (subst; simpl; try omega) : sublist_supp.
+
+  Lemma rejoin_size1: forall n m : Z, n + (m - n) = m.
+  Proof. intros; omega. Qed.
+
+  Lemma rejoin_size2 : forall (n m : nat), (n <= m)%nat -> (n + (m - n))%nat = m.
+  Proof. intros; omega. Qed.
+
+  Hint Rewrite rejoin_size1: sublist_supp.
+  Hint Rewrite rejoin_size2
+       using (apply Nat2Z.inj_le; subst; simpl; try omega) : sublist_supp.
+  
+  Tactic Notation "autorewrite_sublist" :=
+    autorewrite with sublist;
+    autorewrite with sublist_supp.
+
+  Tactic Notation "autorewrite_sublist" "in" ident(H) :=
+    autorewrite with sublist in H;
+    autorewrite with sublist_supp in H.
+  
+  Hint Rewrite add_repr : vst_repr.
+
+  Hint Unfold upd_conn_request : updates.
+  Hint Unfold upd_conn_response : updates.
+  Hint Unfold upd_conn_response_bytes_sent : updates.
+  Hint Unfold upd_conn_state : updates.
+
+  Hint Resolve trace_incl_respects_bind_assoc.
+  Hint Resolve trace_or_incl_bind1.
+  Hint Resolve trace_incl_refl.
+
+End Auto_DB.
+
+Module Protection.
+  Inductive equal {A : Type} (x : A): A -> Prop :=
+  | equal_refl: equal x x.
+
+  Lemma equal_iff : forall (A : Type) (x y : A), x = y <-> equal x y.
+  Proof. intros. split; intros; inversion H; try constructor; auto. Qed.
+
+  Ltac to_equal :=
+    repeat match goal with
+           | [H : _ = _ |- _] =>
+             apply equal_iff in H
+           end.
+
+  Ltac from_equal :=
+    repeat match goal with
+           | [H : equal _ _ |- _] =>
+             apply equal_iff in H
+           end.
+End Protection.
+
+Module Int_Repr.
+        
+  Ltac int_repr_inversion :=
+    match goal with
+    | [|- ?x = ?y] =>
+      match goal with
+      | [H: Int.repr x = Int.repr y |- _] =>
+        apply repr_inj_signed in H;
+        unfold repable_signed;
+        try rep_omega
+      end
+    | [|- ?x <> ?y] =>
+      match goal with
+      | [H: Int.repr x <> Int.repr y |- _] =>
+        apply repr_inj_signed' in H;
+        unfold repable_signed;
+        try rep_omega
+      end    
+    end.
+
+  Ltac int_ineq_to_Z_ineq :=
+    match goal with
+    | [H : context[Int.signed (Int.repr ?r)] |- context[?r] ] =>
+      rewrite Int.signed_repr in H;
+      try rep_omega
+    | [H: Int.repr _ <> Int.repr _ |- _] =>
+      apply repr_neq_e in H
+    end.
+  
+End Int_Repr.
+
+Module Trace_Tactics.
+  (* Introduces hypothesis that left branch of "Or" in current Itree is 
+   included in the current Itree
+   *)
+  Ltac intro_trace_or_incl HTrace left_trace :=
+    match goal with
+    | [|- context[ITREE ?t]] =>
+      match t with
+      | (r <- ?or_trace ;; ?k) =>
+        match or_trace with
+        | Common.or ?t1 ?t2 =>
+          remember t1 as left_trace;
+          assert (trace_incl (r <- t1 ;; k) t)
+            as HTrace
+              by (apply trace_or_incl_bind1)
+        end
+      | Common.or ?t1 ?t2 =>
+        remember t1 as left_trace;
+        assert (trace_incl t1 t) as HTrace
+            by (apply trace_or_incl)
+      end
+    end.
+
+  (* Introduces hypothesis that current Itree is included in itself *)
+  Ltac intro_trace_refl_incl HTrace :=
+    match goal with
+    | [|- context[ITREE ?t]] =>
+      assert (trace_incl t t) as HTrace
+          by (apply trace_incl_refl)
+    end.
+
+  Ltac simpl_trace_incl HTrace :=
+    try apply trace_incl_respects_bind_assoc in HTrace.
+
+  (* Chooses either first or second branch of "Or" *)
+  Ltac take_branch1 idx := 
+    match goal with
+    | [|- context[ITREE (bind (Common.or ?branch1 ?branch2) ?k)]] =>
+      replace_SEP idx (ITREE (r <- branch1 ;; k r));
+      [go_lower; apply internal_nondet1 | ]
+    end.
+
+  Ltac take_branch2 idx := 
+    match goal with
+    | [|- context[ITREE (bind (Common.or ?branch1 ?branch2) ?k)]] =>
+      replace_SEP idx (ITREE (r <- branch2 ;; k r));
+      [go_lower; apply internal_nondet2 | ]
+    end.
+
+  Ltac trace_bind_ret :=
+    match goal with
+    | [|- context[ITREE (bind (ret ?a) ?k)]] =>
+      rewrite (trace_bind_ret a)
+    | [|- context[ITREE (bind (Ret ?a) ?k)]] =>
+      rewrite (trace_bind_ret a)
+    end.
+
+  Ltac rem_trace_tail cont :=
+  match goal with
+  | [ |- context[ITREE (bind _ ?k)]] =>
+    remember k as cont
+  end.
+
+  Ltac rem_trace cont :=
+    match goal with
+    | [ |- context[ITREE ?k]] =>
+      remember k as cont
+    end.
+
+  Ltac rem_trace_or cont1 cont2 cont3 :=
+    match goal with
+    | [|- context[ITREE (bind (or ?k1 ?k2) ?k3)]] =>
+      remember k1 as cont1;
+      remember k2 as cont2;
+      remember k3 as cont3
+    end.
+
+  Ltac unify_trace :=
+    match goal with
+    | [|- derives ?LHS ?RHS] =>
+      match LHS with
+      | context[ITREE ?tr1] =>
+        match RHS with
+        | context[ITREE ?tr2] =>
+          replace tr1 with tr2 by reflexivity
+        end
+      end
+    end.
+  
+End Trace_Tactics.
+
+Module Field_At_Data_At.
+
+  Ltac rem_ptr p :=
+    match goal with
+    | [|- context[SEPx (?data_pred :: _)]] =>
+      match data_pred with
+      | data_at _ _ _ ?ptr =>
+        remember ptr as p 
+      | data_at_ _ _ ?ptr =>
+        remember ptr as p
+      | field_at _ _ _ _ ?ptr =>
+        remember ptr as p
+      | field_at_ _ _ _ ?ptr =>
+        remember ptr as p
+      end
+    end.
+
+  (* Changes first sep conjunct containing data_at to field_at_ *)
+  Ltac data_at_to_field_at :=
+    match goal with
+    | [|- context[SEPx (?data_pred :: ?SP)]] =>
+      match data_pred with
+      | data_at ?sh ?reptype ?rep ?ptr =>
+        replace_SEP 0 (field_at sh reptype [] rep ptr) by entailer!
+      end
+    end.
+
+  (* Changes first sep conjunct containing data_at to field_at with defaults *)
+  Ltac data_at_to_field_at_default :=
+    let to_data_at__ sh reptype ptr :=
+        (replace_SEP
+           0
+           (data_at_ sh reptype ptr) by entailer!) in
+    let to_field_at_default sh reptype ptr :=
+        (replace_SEP
+           0
+           (field_at sh reptype [] (default_val reptype) ptr)
+          by entailer!) in
+    match goal with
+    | [|- context[SEPx (?data_pred :: ?SP)]] =>
+      match data_pred with
+      | data_at ?sh ?reptype ?rep ?ptr =>
+        to_data_at__ sh reptype ptr;
+        to_field_at_default sh reptype ptr
+      | data_at_ ?sh ?reptype ?ptr =>
+        to_field_at_default sh reptype ptr
+      end
+    end.
+
+  (* At first sep conjunct containing a [field_at] with a [field_address] ptr, 
+   rebase it to the head of the structure.
+   *)
+  Ltac field_at_rebase_ptr :=
+    match goal with
+    | [|- context[SEPx (?field_at_pred :: _)]] =>
+      match field_at_pred with
+      | field_at ?sh ?inner_type ?nested_path ?rep
+                 (field_address ?base_type ?path ?ptr) =>
+        replace_SEP
+          0
+          (field_at sh base_type (path ++ nested_path) rep ptr);
+        [go_lower;
+         rewrite field_address_offset; auto;
+         unfold field_at, at_offset;
+         simpl;
+         unfold tarray;
+         try rewrite isptr_offset_val_zero; auto;
+         try entailer! |] 
+      end
+    end.
+
+  Ltac erase_data :=
+    match goal with
+    | [|- context[SEPx (data_at ?sh ?reptype ?rep ?ptr :: _)]] =>
+      replace_SEP
+        0
+        (data_at_ sh reptype ptr) by entailer!
+    end.
+
+  Ltac prove_field_compatible0_array_field_addr :=
+  match goal with
+  | [|- field_compatible0 _ [ArraySubsc _]
+                         (field_address ?reptype ?path ?ptr)] =>
+    eapply field_compatible0_cons_Tarray; [reflexivity | | auto; try omega];
+    let Hcompat := fresh "Hcompat" in
+    pose proof (field_compatible_nested_field reptype path ptr) as Hcompat;
+    try apply Hcompat
+  end.
+
+  Ltac prove_field_compatible_smaller_array :=
+    unfold tarray;
+    match goal with
+    | [|- field_compatible (Tarray _ _ _) ?path ?ptr] =>
+      eapply field_compatible_array_smaller0
+    end.
+  
+End Field_At_Data_At.
+
+Module Buffer_Bounds.
+  
+  (* Introduces bound on representation of contents derived from 
+   a data_at/field_at; assumes such a predicate in first position *)
+  Ltac intro_rep_in_buffer_bound :=
+    unfold tarray;
+    match goal with
+    | [|- context[SEPx (data_at ?sh ?reptype ?rep ?ptr :: _)]] =>
+      match reptype with
+      | Tarray _ ?size _ =>
+        replace_SEP 0 (!! (Zlength rep <= size) && data_at sh reptype rep ptr)
+      end
+    | [|- context[SEPx (field_at ?sh ?reptype ?path ?rep ?ptr :: _)]] =>
+      match reptype with
+      | Tarray _ ?size _ =>
+        replace_SEP 0 (!! (Zlength rep <= size) &&
+                          field_at sh reptype path rep ptr)
+      end
+    end;
+    [ (* go_lower; try derive_buffer_bound *) entailer! | ].
+
+  (* Given [data_at _ _ (rep_msg msg bound) _] in the first position, 
+   saturate context with bounds and equalities that are useful for splitting.
+   *)
+  Ltac saturate_rep_msg_bounds :=
+    match goal with
+    | [|- context[SEPx
+                   (data_at ?sh ?reptype (rep_msg ?msg ?bound) ?ptr :: _)]] =>
+      intro_rep_in_buffer_bound;
+      Intros;
+      match goal with
+      | [H1: Zlength (rep_msg msg _) <= _ |- _] =>
+        pose proof (rep_msg_bound _ _ H1);
+        pose proof (rep_msg_exact_length _ _ H1)
+      end;
+      pose proof (Zlength_nonneg (val_of_string msg))
+    end.
+  
+End Buffer_Bounds.
+
+Module Buffer_Splitting.
+
+  Import Auto_DB.
+  
+  Tactic Notation "split_data_at" :=
+    match goal with
+    | [|- context[SEPx (data_at _ _ (_ ++ _) ?ptr :: _)]] =>
+      first [ unfold tarray;
+              erewrite split_data_app;
+              [ | | reflexivity | autorewrite_sublist; auto];
+              try omega
+            | idtac "Try obtaining bounds for buffer contents"]
+    end.
+
+  Tactic Notation "split_data_at" constr(offset_term) :=
+    match goal with
+    | [|- context[SEPx (data_at _ _ _ ?ptr :: _)]] =>
+      first [ let offset := fresh "offset" in
+              remember offset_term as offset;
+              rewrite split2_data_at_Tarray_tuchar with (n1 := offset);
+              auto; try omega;
+              subst offset
+            | idtac "Try obtaining bounds for buffer contents"]
+    end.
+  
+End Buffer_Splitting.
+
+Module Buffer_Coalescing.
+  Import Auto_DB.
+
+  (* 
+     Finds terms of the form [... ++ list_repeat ... Vundef] and tries to 
+     turn it into [rep_msg str] for some str.
+   *)
+  Ltac fold_rep_msg :=
+    let replace_tac rep msg bound :=
+        (replace rep with (rep_msg msg bound);
+         [| unfold BUFFER_SIZE; unfold rep_msg;
+            autorewrite_sublist; auto])
+    in
+    match goal with
+    | [|- context[sublist ?m ?n (rep_msg ?msg ?bound)
+                         ++ list_repeat ?c Vundef]] =>
+      replace_tac (sublist m n (rep_msg msg bound) ++ list_repeat c Vundef)
+                  msg bound
+    (* | [|- context [val_of_string ?msg1 ++ val_of_string ?msg2
+                                ++ list_repeat ?undef_len Vundef]] =>
+      replace_tac (val_of_string msg1 ++ val_of_string msg2
+                                 ++ list_repeat undef_len Vundef)
+                  (msg1 ++ msg2)%string
+                  (Zlength (val_of_string ((msg1 ++ msg2)%string))
+                   + Z.of_nat undef_len) *)
+    | [|- context [val_of_string ?msg ++ list_repeat ?undef_len Vundef]] =>
+      replace_tac (val_of_string msg ++ list_repeat undef_len Vundef)
+                  msg (Zlength (val_of_string msg) + Z.of_nat undef_len)
+    end;
+    autorewrite_sublist.
+
+  (* Assumes a first sep conjunct of the forms :
+     - [data_at ... * data_at ...]
+     - [data_at ... * data_at_ ...]
+     Rejoins into a single [data_at ...].
+  *)
+  Ltac coalesce :=
+    let pre := (unfold tarray; unfold rep_msg) in
+    (* let post := (autorewrite_sublist; try fold_rep_msg) in *)
+    match goal with
+    | [|- context[SEPx (?data_pred :: _)]] =>
+      match data_pred with
+      | data_at _ _ _ ?ptr * data_at _ _ _ (field_address0 _ _ ?ptr) =>
+        let new_data_pred := fresh "new_data" in
+        pre;
+        evar (new_data_pred : mpred);
+        replace_SEP 0 new_data_pred;
+        [ go_lower; rewrite <- split_data_app;
+          (* simplify before unification + simplify to solve constraints *)
+          autorewrite_sublist; 
+          [ subst new_data_pred; apply derives_refl
+          | auto; try omega..]
+        |
+        ]; subst new_data_pred 
+      | data_at _ _ _ ?ptr * data_at_ _ _ (field_address0 _ _ ?ptr) =>
+        let new_data_pred := fresh "new_data" in        
+        pre;
+        evar (new_data_pred : mpred);
+        replace_SEP 0 new_data_pred;
+        [ go_lower;
+          erewrite <- split_data_with_undefined_tail;
+          autorewrite_sublist;
+          [ | | | reflexivity];
+          [subst new_data_pred; apply derives_refl
+          | auto; try omega ..]
+        |
+        ]; subst new_data_pred
+      end
+    end.
+  
+End Buffer_Coalescing.
+
+Section Deprecated.
+
+  Import Protection.
+  Import Trace_Tactics.
+
+  Ltac forward_if_with conjunct := 
+    match goal with
+    | [|- semax _
+               (PROPx ?Props
+                      (LOCALx ?Locals
+                              (SEPx ?SP))) _ _] =>
+      forward_if (PROPx (conjunct :: Props)
+                        (LOCALx Locals
+                                (SEPx SP)))
+    end.
+      
+  Ltac bool_ineq_to_prop :=
+    match goal with
+    | [|- ~(?LHS > ?RHS)] =>
+      match goal with
+      | [H: LHS >? RHS = false |- _] =>
+        unfold not; intros Hnot;
+        rewrite Zgt_is_gt_bool in Hnot;
+        rewrite Hnot in H; inversion H
+      end
+    | [|- ?LHS > ?RHS] =>
+      match goal with
+      | [H : LHS >? RHS = true |- _] =>
+        rewrite Zgt_is_gt_bool; auto
+      end
+    | [|- ?LHS <= ?RHS] =>
+      match goal with
+      | [H : LHS <=? RHS = true |- _] =>
+        rewrite Zle_is_le_bool; auto
+      end
+    | [|- ~(?LHS <= ?RHS)] =>
+      match goal with
+      | [H: LHS <=? RHS = false |- _] =>
+        unfold not; intros Hnot;
+        rewrite Zle_is_le_bool in Hnot;
+        rewrite Hnot in H; inversion H
+      end
+    end.
+
+  Tactic Notation "seal_entailer" :=
+    let cont := fresh "cont" in
+    (try rem_trace cont; to_equal; entailer!; from_equal; try subst cont).
+
+  Tactic Notation "seal_forward" tactic(tac) :=
+    let cont := fresh "cont" in  
+    (try rem_trace cont; to_equal; tac; from_equal; try subst cont).
+
+
+  Ltac cases_on_ret return_val :=
+    let yes_no_disj_tac H :=
+        let ret_ineq := fresh "ret_ineq" in
+        destruct H;
+        try assert (return_val >= 0) as ret_ineq
+            by omega;
+        try assert (return_val < 0) as ret_ineq
+            by omega
+    in
+    match goal with
+    | [H: ?lhs \/ ?rhs |- _] =>
+      match lhs with
+      | context[return_val] =>
+        unfold YES, NO in *;
+        yes_no_disj_tac H;
+        match goal with
+        | [H1: return_val >= 0, 
+           H2: return_val >= 0 -> _,
+           H3: return_val < 0 -> _ |- _] =>
+          pose proof (H2 H1); clear H1 H2 H3
+        | [H1: return_val < 0, 
+           H2: return_val < 0 -> _,
+           H3: return_val >= 0 -> _ |- _] =>
+          pose proof (H2 H1); clear H1 H2 H3
+        | [H1: return_val <> 0, 
+           H2: return_val <> 0 -> _,
+           H3: return_val = 0 -> _ |- _] =>
+          pose proof (H2 H1); clear H1 H2 H3 
+        | [H1: return_val = 0, 
+           H2: return_val = 0 -> _,
+           H3: return_val <> 0 -> _ |- _] =>
+          pose proof (H2 H1); clear H1 H2 H3
+        end
+      end
+    end.
+
+  
+  Ltac apply_data_array_at_local_facts :=
+    match goal with
+    | [|- context[data_at ?sh (Tarray tuchar ?size ?attr)
+                         ?contents ?ptr]] =>
+      (* 
+    Alternatives:
+    let Hderives := fresh "Hderives" in
+    pose proof data_array_at_local_facts as Hderives;
+
+    match goal with
+    | [H: _ |-- !! ?RHS |- _] =>
+      assert_PROP RHS; [apply Hderives |]
+    end.
+    
+    eapply assert_PROP'; [apply Hderives |].
+       *)
+      sep_apply (data_array_at_local_facts tuchar size attr sh contents ptr)
+    end.
+
+  (* Solves a constraint of the form introduced by [intro_rep_in_buffer_bound] 
+   *)
+  Ltac derive_buffer_bound :=
+    intros;
+    apply andp_right; [| cancel];  
+    try rewrite field_at_data_at;
+    try rewrite field_address_offset;
+    auto;
+    simpl;
+    unfold tarray;
+    try apply_data_array_at_local_facts; 
+    unfold unfold_reptype;
+    simpl;
+    try entailer.
+
+End Deprecated.
+
+Export Auto_DB.
+Export Protection.
+Export Int_Repr.
+Export Trace_Tactics.
+Export Field_At_Data_At.
+Export Buffer_Bounds.
+Export Buffer_Splitting.
+Export Buffer_Coalescing.
