dw/DeepWeb/Spec/ServerDefs.v
@@ -2,8 +2,9 @@ Require Import Coq.ZArith.ZArith.
 Open Scope Z.
 
 From Custom Require Import String.
+Require Import DeepWeb.Lib.Util.
 
 Definition BUFFER_SIZE : Z := 1024.
-Definition SERVER_PORT : Z := 8000.
+Definition SERVER_PORT : endpoint_id := Endpoint 8000.
 
 Definition INIT_MSG := repeat_string "0"%char (Z.to_nat BUFFER_SIZE).
