dw/DeepWeb/Spec/Vst/AppLogic.v
@@ -1,0 +1,179 @@
+Require Import String.
+
+From DeepWeb.Lib Require Import
+     VstLib.
+
+From DeepWeb.Spec Require Import
+     Vst.MainInit
+     Vst.SocketSpecs
+     Swap_CLikeSpec.
+
+Require Import DeepWeb.Lib.VstLib.
+
+Import SockAPIPred.
+Import TracePred.
+
+Open Scope logic.
+Open Scope list.
+
+Set Bullet Behavior "Strict Subproofs".
+
+(***************************** Application Logic ******************************)
+
+Inductive recv_step (buffer_size : Z):
+  (connection * sockfd * SocketMap * string) ->
+  (connection * sockfd * SocketMap * string) -> Prop :=
+| Conn_RECVING_RECVING:
+    forall (conn : connection) (fd : sockfd) (sock_st : SocketMap)
+      (msg_in_store : string)
+      (recved_msg : string)
+      (conn' : connection),
+      conn_state conn = RECVING ->
+      conn' = {| conn_id := conn_id conn;
+                 conn_request := (conn_request conn) ++ recved_msg;
+                 conn_response := conn_response conn;
+                 conn_response_bytes_sent := conn_response_bytes_sent conn;
+                 conn_state := RECVING
+              |} ->
+      lookup_socket sock_st fd = ConnectedSocket (conn_id conn) ->
+      recv_step buffer_size
+                (conn, fd, sock_st, msg_in_store)
+                (conn', fd, sock_st, msg_in_store)
+| Conn_RECVING_SENDING:
+    forall (conn : connection) (fd : sockfd) (sock_st : SocketMap)
+      (msg_in_store : string)
+      (recved_msg : string)
+      (conn' : connection),
+      let full_request := (conn_request conn ++ recved_msg)%string in
+      conn_state conn = RECVING ->
+      is_complete buffer_size full_request = true ->
+      conn' = {| conn_id := conn_id conn;
+                 conn_request := full_request;
+                 conn_response := msg_in_store;
+                 conn_response_bytes_sent := 0;
+                 conn_state := SENDING
+              |} ->
+      lookup_socket sock_st fd = ConnectedSocket (conn_id conn) ->
+      recv_step buffer_size
+                (conn, fd, sock_st, msg_in_store)
+                (conn', fd, sock_st, full_request)
+| Conn_RECVING_EOF:
+    forall (conn : connection) (fd : sockfd) (sock_st : SocketMap)
+      (msg_in_store : string)
+      (conn' : connection) (sock_st' : SocketMap),
+      conn_state conn = RECVING ->
+      conn' = {| conn_id := conn_id conn;
+                 conn_request := conn_request conn;
+                 conn_response := conn_response conn;
+                 conn_response_bytes_sent := conn_response_bytes_sent conn;
+                 conn_state := DELETED
+              |} ->
+      lookup_socket sock_st fd = ConnectedSocket (conn_id conn) ->
+      sock_st' = update_socket_state sock_st fd OpenedSocket ->
+      recv_step buffer_size
+                (conn, fd, sock_st, msg_in_store)
+                (conn', fd, sock_st', msg_in_store)
+| Conn_RECVING_Id:
+    forall (conn : connection) (fd : sockfd) (sock_st : SocketMap)
+      (msg_in_store : string), 
+      recv_step buffer_size
+                (conn, fd, sock_st, msg_in_store)
+                (conn, fd, sock_st, msg_in_store).
+
+
+Inductive send_step:
+  (connection * sockfd * SocketMap) ->
+  (connection * sockfd * SocketMap) -> Prop :=
+| Conn_SENDING_SENDING:
+    forall (conn : connection) (fd : sockfd) (sock_st : SocketMap)
+      (num_bytes_sent : Z) (conn' : connection),
+      conn_state conn = SENDING ->
+      num_bytes_sent >= 0 ->
+      let response_length := Zlength (val_of_string (conn_response conn)) in
+      let total_num_bytes_sent :=
+          conn_response_bytes_sent conn + num_bytes_sent in
+      total_num_bytes_sent < response_length ->
+      conn' = {| conn_id := conn_id conn;
+                 conn_request := conn_request conn;
+                 conn_response := conn_response conn;
+                 conn_response_bytes_sent := total_num_bytes_sent;
+                 conn_state := SENDING
+              |} ->
+      lookup_socket sock_st fd = ConnectedSocket (conn_id conn) ->
+      send_step (conn, fd, sock_st) (conn', fd, sock_st)
+| Conn_SENDING_RECVING:
+    forall (conn : connection) (fd : sockfd) (sock_st : SocketMap)
+      (num_bytes_sent : Z) (conn' : connection),
+      conn_state conn = SENDING ->
+      let response_length := Zlength (val_of_string (conn_response conn)) in
+      let total_num_bytes_sent :=
+          conn_response_bytes_sent conn + num_bytes_sent in
+      total_num_bytes_sent = response_length ->
+      conn' = {| conn_id := conn_id conn;
+                 conn_request := "";
+                 conn_response := "";
+                 conn_response_bytes_sent := 0;
+                 conn_state := RECVING
+              |} ->
+      lookup_socket sock_st fd = ConnectedSocket (conn_id conn) ->
+      send_step (conn, fd, sock_st) (conn', fd, sock_st)
+| Conn_SENDING_Fail:
+    forall (conn : connection) (fd : sockfd) (sock_st : SocketMap)
+      (conn' : connection) (sock_st' : SocketMap),
+      conn' = {| conn_id := conn_id conn;
+                 conn_request := conn_request conn;
+                 conn_response := conn_response conn;
+                 conn_response_bytes_sent := conn_response_bytes_sent conn;
+                 conn_state := DELETED
+              |} ->
+      (sock_st' = sock_st \/
+       sock_st' = update_socket_state sock_st fd OpenedSocket) ->
+      send_step (conn, fd, sock_st) (conn', fd, sock_st').
+
+
+Inductive consistent_state (buffer_size : Z)
+  : SocketMap -> (connection * sockfd) -> Prop :=
+| Consistent_RECVING:
+    forall (client_fd : sockfd) (client_id : connection_id) (request : string)
+      (conn: connection) (sock_st : SocketMap),
+      descriptor (client_fd) < FD_SETSIZE ->
+      conn = {| conn_id := client_id ;
+                conn_request := request;
+                conn_response := "";
+                conn_response_bytes_sent := 0;
+                conn_state := RECVING
+             |} ->
+      lookup_socket sock_st client_fd = ConnectedSocket client_id ->
+      consistent_state buffer_size sock_st (conn, client_fd)
+| Consistent_SENDING:
+    forall (client_fd : sockfd) (client_id : connection_id)
+      (request : string) (response: string) (num_bytes_sent : Z)
+      (conn: connection) (sock_st : SocketMap),
+      descriptor (client_fd) < FD_SETSIZE ->
+      conn = {| conn_id := client_id ;
+                conn_request := request;
+                conn_response := response;
+                conn_response_bytes_sent := num_bytes_sent;
+                conn_state := SENDING
+             |} ->
+      lookup_socket sock_st client_fd = ConnectedSocket client_id ->
+      is_complete buffer_size request = true ->
+      0 <= num_bytes_sent <= Zlength (val_of_string response) ->      
+      consistent_state buffer_size sock_st (conn, client_fd)
+| Consistent_DELETED:
+    forall (client_fd : sockfd) (client_id : connection_id)
+      (request : string) (response : string)
+      (num_bytes_sent : Z)
+      (conn: connection) (sock_st : SocketMap),
+      descriptor client_fd < FD_SETSIZE ->
+      conn = {| conn_id := client_id;
+                conn_request := request;
+                conn_response := response;
+                conn_response_bytes_sent := num_bytes_sent;
+                conn_state := DELETED
+             |} ->
+      (lookup_socket sock_st client_fd = OpenedSocket \/
+       lookup_socket sock_st client_fd = ConnectedSocket client_id) ->
+      0 <= num_bytes_sent <= Zlength (val_of_string response) ->
+      consistent_state buffer_size sock_st (conn, client_fd).
+
