dw/DeepWeb/Spec/Vst/MainInit.v
@@ -1,0 +1,15 @@
+Require Export VST.floyd.proofauto.
+Require Export VST.floyd.library.
+Require Export VST.progs.list_dt.
+Export LsegGeneral.
+
+Require Export DeepWeb.Spec.main.
+Require Export DeepWeb.Spec.ServerDefs.
+
+Instance CompSpecs : compspecs. make_compspecs prog. Defined.
+
+Lemma buffer_size_bounds: 0 < BUFFER_SIZE < Int.max_signed.
+Proof.
+  unfold BUFFER_SIZE.
+  rep_omega.
+Qed.
