dw/DeepWeb/Spec/main.v
@@ -3,7 +3,7 @@ From compcert Require Import Coqlib Integers Floats AST Ctypes Cop Clight Clight
 Local Open Scope Z_scope.
 
 Definition _fd_set : ident := 15%positive.
-Definition ___arr : ident := 101%positive.
+Definition ___arr : ident := 100%positive.
 Definition ___builtin_annot : ident := 34%positive.
 Definition ___builtin_annot_intval : ident := 35%positive.
 Definition ___builtin_bswap : ident := 28%positive.
@@ -56,136 +56,117 @@ Definition ___compcert_va_float64 : ident := 43%positive.
 Definition ___compcert_va_int32 : ident := 41%positive.
 Definition ___compcert_va_int64 : ident := 42%positive.
 Definition ___fds_bits : ident := 14%positive.
-Definition ___i : ident := 100%positive.
-Definition ___stringlit_1 : ident := 158%positive.
-Definition ___stringlit_2 : ident := 159%positive.
-Definition _accept : ident := 90%positive.
-Definition _accept_connection : ident := 133%positive.
-Definition _add_to_fd_set : ident := 136%positive.
-Definition _addr : ident := 156%positive.
-Definition _addr_len : ident := 157%positive.
-Definition _argc : ident := 154%positive.
-Definition _argv : ident := 155%positive.
-Definition _atoi : ident := 79%positive.
-Definition _bind : ident := 86%positive.
-Definition _buffer : ident := 109%positive.
-Definition _buffer_ptr : ident := 94%positive.
-Definition _check_if_complete : ident := 106%positive.
-Definition _close : ident := 84%positive.
-Definition _complete : ident := 120%positive.
-Definition _conn : ident := 111%positive.
-Definition _conn_fd : ident := 117%positive.
-Definition _conn_read : ident := 122%positive.
-Definition _conn_st : ident := 128%positive.
-Definition _conn_write : ident := 127%positive.
+Definition ___i : ident := 99%positive.
+Definition _accept : ident := 89%positive.
+Definition _accept_connection : ident := 132%positive.
+Definition _add_to_fd_set : ident := 135%positive.
+Definition _addr : ident := 153%positive.
+Definition _addr_len : ident := 156%positive.
+Definition _argc : ident := 159%positive.
+Definition _argv : ident := 160%positive.
+Definition _bind : ident := 85%positive.
+Definition _bind_socket : ident := 157%positive.
+Definition _buffer : ident := 108%positive.
+Definition _buffer_ptr : ident := 93%positive.
+Definition _check_if_complete : ident := 105%positive.
+Definition _close : ident := 83%positive.
+Definition _complete : ident := 119%positive.
+Definition _conn : ident := 110%positive.
+Definition _conn_fd : ident := 116%positive.
+Definition _conn_read : ident := 121%positive.
+Definition _conn_st : ident := 127%positive.
+Definition _conn_write : ident := 126%positive.
 Definition _connection : ident := 23%positive.
-Definition _curr : ident := 139%positive.
-Definition _curr_fd : ident := 141%positive.
-Definition _curr_st : ident := 140%positive.
-Definition _es : ident := 148%positive.
+Definition _curr : ident := 138%positive.
+Definition _curr_fd : ident := 140%positive.
+Definition _curr_st : ident := 139%positive.
+Definition _es : ident := 147%positive.
+Definition _exit : ident := 80%positive.
 Definition _fd : ident := 16%positive.
-Definition _fd_clr_macro : ident := 104%positive.
-Definition _fd_isset_macro : ident := 103%positive.
-Definition _fd_set_macro : ident := 105%positive.
-Definition _fd_zero_macro : ident := 102%positive.
-Definition _flags : ident := 96%positive.
-Definition _head : ident := 131%positive.
-Definition _htons : ident := 92%positive.
+Definition _fd_clr_macro : ident := 103%positive.
+Definition _fd_isset_macro : ident := 102%positive.
+Definition _fd_set_macro : ident := 104%positive.
+Definition _fd_zero_macro : ident := 101%positive.
+Definition _flags : ident := 95%positive.
+Definition _head : ident := 130%positive.
+Definition _htons : ident := 91%positive.
 Definition _in_addr : ident := 5%positive.
-Definition _last_msg : ident := 113%positive.
-Definition _last_msg_len : ident := 114%positive.
-Definition _last_msg_store : ident := 112%positive.
-Definition _len : ident := 95%positive.
-Definition _listen : ident := 89%positive.
-Definition _main : ident := 160%positive.
-Definition _malloc : ident := 80%positive.
-Definition _max_fd : ident := 134%positive.
-Definition _maxsock : ident := 150%positive.
+Definition _init_store : ident := 158%positive.
+Definition _last_msg : ident := 112%positive.
+Definition _last_msg_len : ident := 113%positive.
+Definition _last_msg_store : ident := 111%positive.
+Definition _len : ident := 94%positive.
+Definition _listen : ident := 88%positive.
+Definition _main : ident := 161%positive.
+Definition _malloc : ident := 79%positive.
+Definition _max_fd : ident := 133%positive.
+Definition _maxsock : ident := 149%positive.
 Definition _memcpy : ident := 81%positive.
 Definition _memset : ident := 82%positive.
-Definition _monitor_connections : ident := 142%positive.
-Definition _new_connection : ident := 108%positive.
-Definition _new_len : ident := 119%positive.
-Definition _new_store : ident := 110%positive.
+Definition _monitor_connections : ident := 141%positive.
+Definition _new_connection : ident := 107%positive.
+Definition _new_len : ident := 118%positive.
+Definition _new_store : ident := 109%positive.
 Definition _next : ident := 24%positive.
 Definition _num_bytes_sent : ident := 21%positive.
-Definition _num_bytes_to_send : ident := 126%positive.
-Definition _num_ready : ident := 152%positive.
-Definition _old_head : ident := 132%positive.
-Definition _populate_response : ident := 115%positive.
-Definition _process : ident := 129%positive.
-Definition _process_connections : ident := 146%positive.
-Definition _ptr : ident := 118%positive.
-Definition _r : ident := 116%positive.
-Definition _read_socket_ready : ident := 144%positive.
-Definition _recv : ident := 88%positive.
-Definition _recv_msg : ident := 97%positive.
-Definition _request : ident := 123%positive.
+Definition _num_bytes_to_send : ident := 125%positive.
+Definition _num_ready : ident := 151%positive.
+Definition _old_head : ident := 131%positive.
+Definition _populate_response : ident := 114%positive.
+Definition _port : ident := 155%positive.
+Definition _process : ident := 128%positive.
+Definition _process_connections : ident := 145%positive.
+Definition _ptr : ident := 117%positive.
+Definition _r : ident := 115%positive.
+Definition _read_socket_ready : ident := 143%positive.
+Definition _recv : ident := 87%positive.
+Definition _recv_msg : ident := 96%positive.
+Definition _request : ident := 122%positive.
 Definition _request_buffer : ident := 18%positive.
 Definition _request_len : ident := 17%positive.
-Definition _reset_connection : ident := 125%positive.
-Definition _response : ident := 124%positive.
+Definition _reset_connection : ident := 124%positive.
+Definition _response : ident := 123%positive.
 Definition _response_buffer : ident := 20%positive.
 Definition _response_len : ident := 19%positive.
-Definition _response_ok : ident := 121%positive.
-Definition _result : ident := 107%positive.
-Definition _rs : ident := 137%positive.
+Definition _response_ok : ident := 120%positive.
+Definition _result : ident := 106%positive.
+Definition _rs : ident := 136%positive.
 Definition _s_addr : ident := 4%positive.
 Definition _sa_data : ident := 2%positive.
 Definition _sa_family : ident := 1%positive.
-Definition _select : ident := 93%positive.
-Definition _select_loop : ident := 153%positive.
-Definition _send : ident := 87%positive.
-Definition _send_msg : ident := 98%positive.
-Definition _server_socket : ident := 147%positive.
-Definition _set : ident := 99%positive.
-Definition _shutdown : ident := 91%positive.
+Definition _select : ident := 92%positive.
+Definition _select_loop : ident := 152%positive.
+Definition _send : ident := 86%positive.
+Definition _send_msg : ident := 97%positive.
+Definition _server_socket : ident := 146%positive.
+Definition _set : ident := 98%positive.
+Definition _shutdown : ident := 90%positive.
 Definition _sin_addr : ident := 8%positive.
 Definition _sin_family : ident := 6%positive.
 Definition _sin_port : ident := 7%positive.
 Definition _sin_zero : ident := 9%positive.
 Definition _sockaddr : ident := 3%positive.
 Definition _sockaddr_in : ident := 10%positive.
-Definition _socket : ident := 85%positive.
-Definition _socket__1 : ident := 130%positive.
-Definition _socket_ready : ident := 143%positive.
+Definition _socket : ident := 84%positive.
+Definition _socket__1 : ident := 129%positive.
+Definition _socket_ready : ident := 142%positive.
 Definition _st : ident := 22%positive.
 Definition _store : ident := 27%positive.
 Definition _stored_msg : ident := 26%positive.
 Definition _stored_msg_len : ident := 25%positive.
-Definition _strcpy : ident := 83%positive.
-Definition _timeout : ident := 149%positive.
+Definition _timeout : ident := 148%positive.
 Definition _timeval : ident := 13%positive.
-Definition _tmp : ident := 135%positive.
-Definition _tmp_head : ident := 151%positive.
+Definition _tmp : ident := 134%positive.
+Definition _tmp_head : ident := 150%positive.
 Definition _tv_sec : ident := 11%positive.
 Definition _tv_usec : ident := 12%positive.
-Definition _write_socket_ready : ident := 145%positive.
-Definition _ws : ident := 138%positive.
-Definition _t'1 : ident := 161%positive.
-Definition _t'2 : ident := 162%positive.
-Definition _t'3 : ident := 163%positive.
-Definition _t'4 : ident := 164%positive.
-Definition _t'5 : ident := 165%positive.
-Definition _t'6 : ident := 166%positive.
-
-Definition v___stringlit_2 := {|
-  gvar_info := (tarray tschar 5);
-  gvar_init := (Init_int8 (Int.repr 116) :: Init_int8 (Int.repr 101) ::
-                Init_int8 (Int.repr 115) :: Init_int8 (Int.repr 116) ::
-                Init_int8 (Int.repr 0) :: nil);
-  gvar_readonly := true;
-  gvar_volatile := false
-|}.
-
-Definition v___stringlit_1 := {|
-  gvar_info := (tarray tschar 5);
-  gvar_init := (Init_int8 (Int.repr 56) :: Init_int8 (Int.repr 48) ::
-                Init_int8 (Int.repr 48) :: Init_int8 (Int.repr 48) ::
-                Init_int8 (Int.repr 0) :: nil);
-  gvar_readonly := true;
-  gvar_volatile := false
-|}.
+Definition _write_socket_ready : ident := 144%positive.
+Definition _ws : ident := 137%positive.
+Definition _zeroize_addr : ident := 154%positive.
+Definition _t'1 : ident := 162%positive.
+Definition _t'2 : ident := 163%positive.
+Definition _t'3 : ident := 164%positive.
+Definition _t'4 : ident := 165%positive.
 
 Definition f_recv_msg := {|
   fn_return := tint;
@@ -1377,140 +1358,202 @@ Definition f_select_loop := {|
             (Sreturn (Some (Econst_int (Int.repr 0) tint)))))))))
 |}.
 
-Definition f_main := {|
+Definition f_zeroize_addr := {|
+  fn_return := tvoid;
+  fn_callconv := cc_default;
+  fn_params := ((_addr, (tptr (Tstruct _sockaddr_in noattr))) :: nil);
+  fn_vars := nil;
+  fn_temps := nil;
+  fn_body :=
+(Scall None
+  (Evar _memset (Tfunction
+                  (Tcons (tptr tvoid) (Tcons tint (Tcons tuint Tnil)))
+                  (tptr tvoid) cc_default))
+  ((Etempvar _addr (tptr (Tstruct _sockaddr_in noattr))) ::
+   (Econst_int (Int.repr 0) tint) ::
+   (Esizeof (Tstruct _sockaddr_in noattr) tuint) :: nil))
+|}.
+
+Definition f_bind_socket := {|
   fn_return := tint;
   fn_callconv := cc_default;
-  fn_params := ((_argc, tint) :: (_argv, (tptr (tptr tschar))) :: nil);
+  fn_params := ((_fd, tint) :: (_port, tint) :: nil);
   fn_vars := ((_addr, (Tstruct _sockaddr_in noattr)) :: nil);
-  fn_temps := ((_addr_len, tint) :: (_fd, tint) :: (_r, tint) ::
-               (_last_msg_store, (tptr (Tstruct _store noattr))) ::
-               (_last_msg, (tptr tschar)) ::
-               (_t'6, (tptr (Tstruct _store noattr))) :: (_t'5, tint) ::
-               (_t'4, tint) :: (_t'3, tint) :: (_t'2, tushort) ::
-               (_t'1, tint) :: nil);
+  fn_temps := ((_addr_len, tint) :: (_r, tint) :: (_t'2, tint) ::
+               (_t'1, tushort) :: nil);
   fn_body :=
 (Ssequence
+  (Scall None
+    (Evar _zeroize_addr (Tfunction
+                          (Tcons (tptr (Tstruct _sockaddr_in noattr)) Tnil)
+                          tvoid cc_default))
+    ((Eaddrof (Evar _addr (Tstruct _sockaddr_in noattr))
+       (tptr (Tstruct _sockaddr_in noattr))) :: nil))
   (Ssequence
+    (Sset _addr_len (Esizeof (Tstruct _sockaddr_in noattr) tuint))
+    (Ssequence
+      (Sassign
+        (Efield (Evar _addr (Tstruct _sockaddr_in noattr)) _sin_family
+          tushort) (Econst_int (Int.repr 2) tint))
+      (Ssequence
+        (Ssequence
+          (Scall (Some _t'1)
+            (Evar _htons (Tfunction (Tcons tushort Tnil) tushort cc_default))
+            ((Etempvar _port tint) :: nil))
+          (Sassign
+            (Efield (Evar _addr (Tstruct _sockaddr_in noattr)) _sin_port
+              tushort) (Etempvar _t'1 tushort)))
+        (Ssequence
+          (Ssequence
+            (Scall (Some _t'2)
+              (Evar _bind (Tfunction
+                            (Tcons tint
+                              (Tcons (tptr (Tstruct _sockaddr noattr))
+                                (Tcons tuint Tnil))) tint cc_default))
+              ((Etempvar _fd tint) ::
+               (Ecast
+                 (Eaddrof (Evar _addr (Tstruct _sockaddr_in noattr))
+                   (tptr (Tstruct _sockaddr_in noattr)))
+                 (tptr (Tstruct _sockaddr noattr))) ::
+               (Etempvar _addr_len tint) :: nil))
+            (Sset _r (Etempvar _t'2 tint)))
+          (Ssequence
+            (Sifthenelse (Ebinop Olt (Etempvar _r tint)
+                           (Econst_int (Int.repr 0) tint) tint)
+              (Sreturn (Some (Eunop Oneg (Econst_int (Int.repr 1) tint) tint)))
+              Sskip)
+            (Sreturn (Some (Econst_int (Int.repr 0) tint)))))))))
+|}.
+
+Definition f_init_store := {|
+  fn_return := tvoid;
+  fn_callconv := cc_default;
+  fn_params := ((_last_msg_store, (tptr (Tstruct _store noattr))) :: nil);
+  fn_vars := nil;
+  fn_temps := ((_last_msg, (tptr tschar)) :: nil);
+  fn_body :=
+(Ssequence
+  (Sassign
+    (Efield
+      (Ederef (Etempvar _last_msg_store (tptr (Tstruct _store noattr)))
+        (Tstruct _store noattr)) _stored_msg_len tuint)
+    (Econst_int (Int.repr 1024) tint))
+  (Ssequence
+    (Sset _last_msg
+      (Ecast
+        (Efield
+          (Ederef (Etempvar _last_msg_store (tptr (Tstruct _store noattr)))
+            (Tstruct _store noattr)) _stored_msg (tarray tuchar 1024))
+        (tptr tschar)))
     (Scall None
       (Evar _memset (Tfunction
                       (Tcons (tptr tvoid) (Tcons tint (Tcons tuint Tnil)))
                       (tptr tvoid) cc_default))
-      ((Eaddrof (Evar _addr (Tstruct _sockaddr_in noattr))
-         (tptr (Tstruct _sockaddr_in noattr))) ::
-       (Econst_int (Int.repr 0) tint) ::
-       (Esizeof (Tstruct _sockaddr_in noattr) tuint) :: nil))
+      ((Etempvar _last_msg (tptr tschar)) ::
+       (Econst_int (Int.repr 48) tint) ::
+       (Econst_int (Int.repr 1024) tint) :: nil))))
+|}.
+
+Definition f_main := {|
+  fn_return := tint;
+  fn_callconv := cc_default;
+  fn_params := ((_argc, tint) :: (_argv, (tptr (tptr tschar))) :: nil);
+  fn_vars := nil;
+  fn_temps := ((_fd, tint) :: (_r, tint) ::
+               (_last_msg_store, (tptr (Tstruct _store noattr))) ::
+               (_port, tint) :: (_t'4, tint) :: (_t'3, tint) ::
+               (_t'2, tint) :: (_t'1, (tptr (Tstruct _store noattr))) :: nil);
+  fn_body :=
+(Ssequence
+  (Ssequence
     (Ssequence
-      (Sset _addr_len (Esizeof (Tstruct _sockaddr_in noattr) tuint))
+      (Scall (Some _t'1)
+        (Evar _new_store (Tfunction Tnil (tptr (Tstruct _store noattr))
+                           cc_default)) nil)
+      (Sset _last_msg_store (Etempvar _t'1 (tptr (Tstruct _store noattr)))))
+    (Ssequence
+      (Sifthenelse (Ebinop Oeq
+                     (Etempvar _last_msg_store (tptr (Tstruct _store noattr)))
+                     (Ecast (Econst_int (Int.repr 0) tint) (tptr tvoid))
+                     tint)
+        (Scall None
+          (Evar _exit (Tfunction (Tcons tint Tnil) tvoid cc_default))
+          ((Econst_int (Int.repr 0) tint) :: nil))
+        Sskip)
       (Ssequence
-        (Sassign
-          (Efield (Evar _addr (Tstruct _sockaddr_in noattr)) _sin_family
-            tushort) (Econst_int (Int.repr 2) tint))
+        (Scall None
+          (Evar _init_store (Tfunction
+                              (Tcons (tptr (Tstruct _store noattr)) Tnil)
+                              tvoid cc_default))
+          ((Etempvar _last_msg_store (tptr (Tstruct _store noattr))) :: nil))
         (Ssequence
           (Ssequence
-            (Ssequence
-              (Scall (Some _t'1)
-                (Evar _atoi (Tfunction (Tcons (tptr tschar) Tnil) tint
-                              cc_default))
-                ((Evar ___stringlit_1 (tarray tschar 5)) :: nil))
-              (Scall (Some _t'2)
-                (Evar _htons (Tfunction (Tcons tushort Tnil) tushort
-                               cc_default)) ((Etempvar _t'1 tint) :: nil)))
-            (Sassign
-              (Efield (Evar _addr (Tstruct _sockaddr_in noattr)) _sin_port
-                tushort) (Etempvar _t'2 tushort)))
+            (Scall (Some _t'2)
+              (Evar _socket (Tfunction
+                              (Tcons tint (Tcons tint (Tcons tint Tnil)))
+                              tint cc_default))
+              ((Econst_int (Int.repr 2) tint) ::
+               (Econst_int (Int.repr 1) tint) ::
+               (Econst_int (Int.repr 0) tint) :: nil))
+            (Sset _fd (Etempvar _t'2 tint)))
           (Ssequence
+            (Sifthenelse (Ebinop Olt (Etempvar _fd tint)
+                           (Econst_int (Int.repr 0) tint) tint)
+              (Scall None
+                (Evar _exit (Tfunction (Tcons tint Tnil) tvoid cc_default))
+                ((Econst_int (Int.repr 0) tint) :: nil))
+              Sskip)
             (Ssequence
-              (Scall (Some _t'3)
-                (Evar _socket (Tfunction
-                                (Tcons tint (Tcons tint (Tcons tint Tnil)))
-                                tint cc_default))
-                ((Econst_int (Int.repr 2) tint) ::
-                 (Econst_int (Int.repr 1) tint) ::
-                 (Econst_int (Int.repr 0) tint) :: nil))
-              (Sset _fd (Etempvar _t'3 tint)))
-            (Ssequence
+              (Sifthenelse (Ebinop Oge (Etempvar _fd tint)
+                             (Econst_int (Int.repr 1024) tint) tint)
+                (Scall None
+                  (Evar _exit (Tfunction (Tcons tint Tnil) tvoid cc_default))
+                  ((Econst_int (Int.repr 0) tint) :: nil))
+                Sskip)
               (Ssequence
-                (Scall (Some _t'4)
-                  (Evar _bind (Tfunction
-                                (Tcons tint
-                                  (Tcons (tptr (Tstruct _sockaddr noattr))
-                                    (Tcons tuint Tnil))) tint cc_default))
-                  ((Etempvar _fd tint) ::
-                   (Ecast
-                     (Eaddrof (Evar _addr (Tstruct _sockaddr_in noattr))
-                       (tptr (Tstruct _sockaddr_in noattr)))
-                     (tptr (Tstruct _sockaddr noattr))) ::
-                   (Etempvar _addr_len tint) :: nil))
-                (Sset _r (Etempvar _t'4 tint)))
-              (Ssequence
-                (Sifthenelse (Ebinop Olt (Etempvar _r tint)
-                               (Econst_int (Int.repr 0) tint) tint)
-                  (Sreturn (Some (Eunop Oneg (Econst_int (Int.repr 1) tint)
-                                   tint)))
-                  Sskip)
+                (Sset _port (Econst_int (Int.repr 8000) tint))
                 (Ssequence
                   (Ssequence
-                    (Scall (Some _t'5)
-                      (Evar _listen (Tfunction (Tcons tint (Tcons tint Tnil))
-                                      tint cc_default))
-                      ((Etempvar _fd tint) ::
-                       (Econst_int (Int.repr 128) tint) :: nil))
-                    (Sset _r (Etempvar _t'5 tint)))
+                    (Scall (Some _t'3)
+                      (Evar _bind_socket (Tfunction
+                                           (Tcons tint (Tcons tint Tnil))
+                                           tint cc_default))
+                      ((Etempvar _fd tint) :: (Etempvar _port tint) :: nil))
+                    (Sset _r (Etempvar _t'3 tint)))
                   (Ssequence
                     (Sifthenelse (Ebinop Olt (Etempvar _r tint)
                                    (Econst_int (Int.repr 0) tint) tint)
-                      (Sreturn (Some (Eunop Oneg
-                                       (Econst_int (Int.repr 1) tint) tint)))
+                      (Scall None
+                        (Evar _exit (Tfunction (Tcons tint Tnil) tvoid
+                                      cc_default))
+                        ((Econst_int (Int.repr 0) tint) :: nil))
                       Sskip)
                     (Ssequence
                       (Ssequence
-                        (Scall (Some _t'6)
-                          (Evar _new_store (Tfunction Tnil
-                                             (tptr (Tstruct _store noattr))
-                                             cc_default)) nil)
-                        (Sset _last_msg_store
-                          (Etempvar _t'6 (tptr (Tstruct _store noattr)))))
+                        (Scall (Some _t'4)
+                          (Evar _listen (Tfunction
+                                          (Tcons tint (Tcons tint Tnil)) tint
+                                          cc_default))
+                          ((Etempvar _fd tint) ::
+                           (Econst_int (Int.repr 128) tint) :: nil))
+                        (Sset _r (Etempvar _t'4 tint)))
                       (Ssequence
-                        (Sifthenelse (Ebinop Oeq
-                                       (Etempvar _last_msg_store (tptr (Tstruct _store noattr)))
-                                       (Ecast (Econst_int (Int.repr 0) tint)
-                                         (tptr tvoid)) tint)
-                          (Sreturn (Some (Econst_int (Int.repr 0) tint)))
+                        (Sifthenelse (Ebinop Olt (Etempvar _r tint)
+                                       (Econst_int (Int.repr 0) tint) tint)
+                          (Scall None
+                            (Evar _exit (Tfunction (Tcons tint Tnil) tvoid
+                                          cc_default))
+                            ((Econst_int (Int.repr 0) tint) :: nil))
                           Sskip)
-                        (Ssequence
-                          (Sassign
-                            (Efield
-                              (Ederef
-                                (Etempvar _last_msg_store (tptr (Tstruct _store noattr)))
-                                (Tstruct _store noattr)) _stored_msg_len
-                              tuint) (Econst_int (Int.repr 5) tint))
-                          (Ssequence
-                            (Sset _last_msg
-                              (Ecast
-                                (Efield
-                                  (Ederef
-                                    (Etempvar _last_msg_store (tptr (Tstruct _store noattr)))
-                                    (Tstruct _store noattr)) _stored_msg
-                                  (tarray tuchar 1024)) (tptr tschar)))
-                            (Ssequence
-                              (Scall None
-                                (Evar _strcpy (Tfunction
-                                                (Tcons (tptr tschar)
-                                                  (Tcons (tptr tschar) Tnil))
-                                                (tptr tschar) cc_default))
-                                ((Etempvar _last_msg (tptr tschar)) ::
-                                 (Evar ___stringlit_2 (tarray tschar 5)) ::
-                                 nil))
-                              (Scall None
-                                (Evar _select_loop (Tfunction
-                                                     (Tcons tint
-                                                       (Tcons
-                                                         (tptr (Tstruct _store noattr))
-                                                         Tnil)) tint
-                                                     cc_default))
-                                ((Etempvar _fd tint) ::
-                                 (Etempvar _last_msg_store (tptr (Tstruct _store noattr))) ::
-                                 nil))))))))))))))))
+                        (Scall None
+                          (Evar _select_loop (Tfunction
+                                               (Tcons tint
+                                                 (Tcons
+                                                   (tptr (Tstruct _store noattr))
+                                                   Tnil)) tint cc_default))
+                          ((Etempvar _fd tint) ::
+                           (Etempvar _last_msg_store (tptr (Tstruct _store noattr))) ::
+                           nil)))))))))))))
   (Sreturn (Some (Econst_int (Int.repr 0) tint))))
 |}.
 
@@ -1538,9 +1581,7 @@ Definition composites : list composite_definition :=
    noattr :: nil).
 
 Definition global_definitions : list (ident * globdef fundef type) :=
-((___stringlit_2, Gvar v___stringlit_2) ::
- (___stringlit_1, Gvar v___stringlit_1) ::
- (___builtin_bswap,
+((___builtin_bswap,
    Gfun(External (EF_builtin "__builtin_bswap"
                    (mksignature (AST.Tint :: nil) (Some AST.Tint) cc_default))
      (Tcons tuint Tnil) tuint cc_default)) ::
@@ -1781,12 +1822,12 @@ Definition global_definitions : list (ident * globdef fundef type) :=
                      {|cc_vararg:=true; cc_unproto:=false; cc_structret:=false|}))
      (Tcons tint Tnil) tvoid
      {|cc_vararg:=true; cc_unproto:=false; cc_structret:=false|})) ::
- (_atoi,
-   Gfun(External (EF_external "atoi"
-                   (mksignature (AST.Tint :: nil) (Some AST.Tint) cc_default))
-     (Tcons (tptr tschar) Tnil) tint cc_default)) ::
  (_malloc,
    Gfun(External EF_malloc (Tcons tuint Tnil) (tptr tvoid) cc_default)) ::
+ (_exit,
+   Gfun(External (EF_external "exit"
+                   (mksignature (AST.Tint :: nil) None cc_default))
+     (Tcons tint Tnil) tvoid cc_default)) ::
  (_memcpy,
    Gfun(External (EF_external "memcpy"
                    (mksignature (AST.Tint :: AST.Tint :: AST.Tint :: nil)
@@ -1798,12 +1839,6 @@ Definition global_definitions : list (ident * globdef fundef type) :=
                    (mksignature (AST.Tint :: AST.Tint :: AST.Tint :: nil)
                      (Some AST.Tint) cc_default))
      (Tcons (tptr tvoid) (Tcons tint (Tcons tuint Tnil))) (tptr tvoid)
-     cc_default)) ::
- (_strcpy,
-   Gfun(External (EF_external "strcpy"
-                   (mksignature (AST.Tint :: AST.Tint :: nil) (Some AST.Tint)
-                     cc_default))
-     (Tcons (tptr tschar) (Tcons (tptr tschar) Tnil)) (tptr tschar)
      cc_default)) ::
  (_close,
    Gfun(External (EF_external "close"
@@ -1885,31 +1920,34 @@ Definition global_definitions : list (ident * globdef fundef type) :=
  (_monitor_connections, Gfun(Internal f_monitor_connections)) ::
  (_process_connections, Gfun(Internal f_process_connections)) ::
  (_select_loop, Gfun(Internal f_select_loop)) ::
+ (_zeroize_addr, Gfun(Internal f_zeroize_addr)) ::
+ (_bind_socket, Gfun(Internal f_bind_socket)) ::
+ (_init_store, Gfun(Internal f_init_store)) ::
  (_main, Gfun(Internal f_main)) :: nil).
 
 Definition public_idents : list ident :=
-(_main :: _select_loop :: _check_if_complete :: _fd_set_macro ::
- _fd_clr_macro :: _fd_isset_macro :: _fd_zero_macro :: _send_msg ::
- _recv_msg :: _select :: _htons :: _shutdown :: _accept :: _listen ::
- _recv :: _send :: _bind :: _socket :: _close :: _strcpy :: _memset ::
- _memcpy :: _malloc :: _atoi :: ___builtin_debug :: ___builtin_nop ::
- ___builtin_write32_reversed :: ___builtin_write16_reversed ::
- ___builtin_read32_reversed :: ___builtin_read16_reversed ::
- ___builtin_fnmsub :: ___builtin_fnmadd :: ___builtin_fmsub ::
- ___builtin_fmadd :: ___builtin_fmin :: ___builtin_fmax ::
- ___builtin_ctzll :: ___builtin_ctzl :: ___builtin_ctz :: ___builtin_clzll ::
- ___builtin_clzl :: ___builtin_clz :: ___builtin_bswap64 ::
- ___compcert_i64_umulh :: ___compcert_i64_smulh :: ___compcert_i64_sar ::
- ___compcert_i64_shr :: ___compcert_i64_shl :: ___compcert_i64_umod ::
- ___compcert_i64_smod :: ___compcert_i64_udiv :: ___compcert_i64_sdiv ::
- ___compcert_i64_utof :: ___compcert_i64_stof :: ___compcert_i64_utod ::
- ___compcert_i64_stod :: ___compcert_i64_dtou :: ___compcert_i64_dtos ::
- ___compcert_va_composite :: ___compcert_va_float64 ::
- ___compcert_va_int64 :: ___compcert_va_int32 :: ___builtin_va_end ::
- ___builtin_va_copy :: ___builtin_va_arg :: ___builtin_va_start ::
- ___builtin_membar :: ___builtin_annot_intval :: ___builtin_annot ::
- ___builtin_memcpy_aligned :: ___builtin_fsqrt :: ___builtin_fabs ::
- ___builtin_bswap16 :: ___builtin_bswap32 :: ___builtin_bswap :: nil).
+(_main :: _select_loop :: _fd_set_macro :: _fd_clr_macro ::
+ _fd_isset_macro :: _fd_zero_macro :: _send_msg :: _recv_msg :: _select ::
+ _htons :: _shutdown :: _accept :: _listen :: _recv :: _send :: _bind ::
+ _socket :: _close :: _memset :: _memcpy :: _exit :: _malloc ::
+ ___builtin_debug :: ___builtin_nop :: ___builtin_write32_reversed ::
+ ___builtin_write16_reversed :: ___builtin_read32_reversed ::
+ ___builtin_read16_reversed :: ___builtin_fnmsub :: ___builtin_fnmadd ::
+ ___builtin_fmsub :: ___builtin_fmadd :: ___builtin_fmin ::
+ ___builtin_fmax :: ___builtin_ctzll :: ___builtin_ctzl :: ___builtin_ctz ::
+ ___builtin_clzll :: ___builtin_clzl :: ___builtin_clz ::
+ ___builtin_bswap64 :: ___compcert_i64_umulh :: ___compcert_i64_smulh ::
+ ___compcert_i64_sar :: ___compcert_i64_shr :: ___compcert_i64_shl ::
+ ___compcert_i64_umod :: ___compcert_i64_smod :: ___compcert_i64_udiv ::
+ ___compcert_i64_sdiv :: ___compcert_i64_utof :: ___compcert_i64_stof ::
+ ___compcert_i64_utod :: ___compcert_i64_stod :: ___compcert_i64_dtou ::
+ ___compcert_i64_dtos :: ___compcert_va_composite ::
+ ___compcert_va_float64 :: ___compcert_va_int64 :: ___compcert_va_int32 ::
+ ___builtin_va_end :: ___builtin_va_copy :: ___builtin_va_arg ::
+ ___builtin_va_start :: ___builtin_membar :: ___builtin_annot_intval ::
+ ___builtin_annot :: ___builtin_memcpy_aligned :: ___builtin_fsqrt ::
+ ___builtin_fabs :: ___builtin_bswap16 :: ___builtin_bswap32 ::
+ ___builtin_bswap :: nil).
 
 Definition prog : Clight.program := 
   mkprogram composites global_definitions public_idents _main Logic.I.
