dw/DeepWeb/Util/MonadNotations.v
@@ -1,4 +1,0 @@
-Generalizable Variable E.
-
-Require Import DeepWeb.Free.Monad.Free.
-Require Import DeepWeb.Util.Common.
