dw/DeepWeb/Util/OptionUtil.v
@@ -1,5 +1,0 @@
-Definition isSome {A} (a: option A): bool :=
-  match a with
-  | Some _ => true
-  | None => false
-  end.
